Slight refactor of pathsync

fstar/MLS.TreeSync.Operations.fst
@@ -67,8 +67,8 @@ let compute_new_np_and_ph #bytes #cb #tkt #l #i opt_ext_content sibling parent_p
   in
   (new_opt_content, new_parent_parent_hash)
 
-val compute_leaf_parent_hash_from_external_path_pre: #bytes:Type0 -> {|crypto_bytes bytes|} -> #tkt:treekem_types bytes -> #l:nat -> #i:tree_index l -> #li:leaf_index l i -> treesync bytes tkt l i -> external_pathsync bytes tkt l i li -> mls_nat -> bool
-let rec compute_leaf_parent_hash_from_external_path_pre #bytes #cb #tkt #l #i #li t p length_parent_parent_hash =
+val compute_leaf_parent_hash_from_external_path_pre: #bytes:Type0 -> {|crypto_bytes bytes|} -> #tkt:treekem_types bytes -> #path_leaf_t:Type -> #l:nat -> #i:tree_index l -> #li:leaf_index l i -> treesync bytes tkt l i -> path path_leaf_t (option tkt.node_content) l i li -> mls_nat -> bool
+let rec compute_leaf_parent_hash_from_external_path_pre #bytes #cb #tkt #path_leaf_t #l #i #li t p length_parent_parent_hash =
   match t, p with
   | TLeaf _, PLeaf _ -> true
   | TNode _ left right, PNode opt_ext_content p_next -> (
@@ -86,10 +86,10 @@ let rec compute_leaf_parent_hash_from_external_path_pre #bytes #cb #tkt #l #i #l
     )
   )
 
-val compute_leaf_parent_hash_from_external_path: #bytes:Type0 -> {|crypto_bytes bytes|} -> #tkt:treekem_types bytes -> #l:nat -> #i:tree_index l -> #li:leaf_index l i -> t:treesync bytes tkt l i -> p:external_pathsync bytes tkt l i li -> parent_parent_hash:mls_bytes bytes -> Pure (mls_bytes bytes)
+val compute_leaf_parent_hash_from_external_path: #bytes:Type0 -> {|crypto_bytes bytes|} -> #tkt:treekem_types bytes -> #path_leaf_t:Type -> #l:nat -> #i:tree_index l -> #li:leaf_index l i -> t:treesync bytes tkt l i -> p:path path_leaf_t (option tkt.node_content) l i li -> parent_parent_hash:mls_bytes bytes -> Pure (mls_bytes bytes)
   (requires compute_leaf_parent_hash_from_external_path_pre t p (length #bytes parent_parent_hash))
   (ensures fun res -> res == parent_parent_hash \/ length #bytes res == hash_length #bytes)
-let rec compute_leaf_parent_hash_from_external_path #bytes #cb #tkt #l #i #li t p parent_parent_hash =
+let rec compute_leaf_parent_hash_from_external_path #bytes #cb #tkt #path_leaf_t #l #i #li t p parent_parent_hash =
   match t, p with
   | TLeaf old_lp, PLeaf new_lp -> parent_parent_hash
   | TNode _ left right, PNode opt_ext_content p_next ->
@@ -100,14 +100,14 @@ let rec compute_leaf_parent_hash_from_external_path #bytes #cb #tkt #l #i #li t 
     else
       compute_leaf_parent_hash_from_external_path right p_next new_parent_parent_hash
 
-val get_external_path_leaf: #bytes:Type0 -> {|crypto_bytes bytes|} -> #tkt:treekem_types bytes -> #l:nat -> #i:tree_index l -> #li:leaf_index l i -> external_pathsync bytes tkt l i li -> leaf_node_nt bytes tkt
-let rec get_external_path_leaf #bytes #cb #tkt #l #i #li p =
+val get_external_path_leaf: #leaf_t:Type -> #node_t:Type -> #l:nat -> #i:tree_index l -> #li:leaf_index l i -> path leaf_t node_t l i li -> leaf_t
+let rec get_external_path_leaf #leaf_t #node_t #i #li p =
   match p with
   | PLeaf lp -> lp
   | PNode _ p_next -> get_external_path_leaf p_next
 
-val set_external_path_leaf: #bytes:Type0 -> {|crypto_bytes bytes|} -> #tkt:treekem_types bytes -> #l:nat -> #i:tree_index l -> #li:leaf_index l i -> external_pathsync bytes tkt l i li -> leaf_node_nt bytes tkt -> external_pathsync bytes tkt l i li
-let rec set_external_path_leaf #bytes #cb #tkt #l #i #li p lp =
+val set_external_path_leaf: #leaf_t_in:Type -> #leaf_t_out:Type -> #node_t:Type -> #l:nat -> #i:tree_index l -> #li:leaf_index l i -> path leaf_t_in node_t l i li -> leaf_t_out -> path leaf_t_out node_t l i li
+let rec set_external_path_leaf #leaf_t_in #leaf_t_out #node_t #l #i #li p lp =
   match p with
   | PLeaf _ -> PLeaf lp
   | PNode p_content p_next -> PNode p_content (set_external_path_leaf p_next lp)
@@ -134,11 +134,11 @@ let leaf_is_valid #bytes #cb #tkt ln group_id leaf_index =
   verify_with_label #bytes ln.data.signature_key "LeafNodeTBS" tbs_bytes ln.signature
   )
 
-val external_path_leaf_is_valid: #bytes:Type0 -> {|crypto_bytes bytes|} -> #tkt:treekem_types bytes -> #l:nat -> #li:leaf_index l 0 -> mls_bytes bytes -> external_pathsync bytes tkt l 0 li -> bool
+val external_path_leaf_is_valid: #bytes:Type0 -> {|crypto_bytes bytes|} -> #tkt:treekem_types bytes -> #l:nat -> #li:leaf_index l 0 -> mls_bytes bytes -> pathsync bytes tkt l 0 li -> bool
 let external_path_leaf_is_valid #bytes #cb #tkt #l #li group_id p =
   leaf_is_valid (get_external_path_leaf p) group_id li
 
-val external_path_is_parent_hash_valid: #bytes:Type0 -> {|crypto_bytes bytes|} -> #tkt:treekem_types bytes -> #l:nat -> #li:leaf_index l 0 -> treesync bytes tkt l 0 -> external_pathsync bytes tkt l 0 li -> bool
+val external_path_is_parent_hash_valid: #bytes:Type0 -> {|crypto_bytes bytes|} -> #tkt:treekem_types bytes -> #l:nat -> #li:leaf_index l 0 -> treesync bytes tkt l 0 -> pathsync bytes tkt l 0 li -> bool
 let external_path_is_parent_hash_valid #bytes #cb #tkt #l #li t p =
   let new_lp = get_external_path_leaf p in
   compute_leaf_parent_hash_from_external_path_pre t p (length #bytes (root_parent_hash #bytes)) && (
@@ -146,7 +146,7 @@ let external_path_is_parent_hash_valid #bytes #cb #tkt #l #li t p =
   (new_lp.data.source = LNS_commit () && (new_lp.data.parent_hash <: bytes) = computed_parent_hash)
   )
 
-val external_path_is_filter_valid: #bytes:Type0 -> {|crypto_bytes bytes|} -> #tkt:treekem_types bytes -> #l:nat -> #i:tree_index l -> #li:leaf_index l i -> treesync bytes tkt l i -> external_pathsync bytes tkt l i li -> bool
+val external_path_is_filter_valid: #bytes:Type0 -> {|crypto_bytes bytes|} -> #tkt:treekem_types bytes -> #l:nat -> #i:tree_index l -> #li:leaf_index l i -> treesync bytes tkt l i -> pathsync bytes tkt l i li -> bool
 let rec external_path_is_filter_valid #bytes #cb #tkt #l #i #li t p =
   match t, p with
   | TLeaf _, PLeaf _ -> true
@@ -160,7 +160,7 @@ let rec external_path_is_filter_valid #bytes #cb #tkt #l #i #li t p =
     sibling_ok && external_path_is_filter_valid child p_next
   )
 
-val external_path_is_valid: #bytes:Type0 -> {|crypto_bytes bytes|} -> #tkt:treekem_types bytes -> #l:nat -> #li:leaf_index l 0 -> mls_bytes bytes -> t:treesync bytes tkt l 0 -> external_pathsync bytes tkt l 0 li -> bool
+val external_path_is_valid: #bytes:Type0 -> {|crypto_bytes bytes|} -> #tkt:treekem_types bytes -> #l:nat -> #li:leaf_index l 0 -> mls_bytes bytes -> t:treesync bytes tkt l 0 -> pathsync bytes tkt l 0 li -> bool
 let external_path_is_valid #bytes #cb #tkt #l #li group_id t p =
   let old_lp = leaf_at t li in
   let new_lp = get_external_path_leaf p in
@@ -176,26 +176,26 @@ val external_path_to_valid_external_path_pre: #bytes:Type0 -> {|crypto_bytes byt
 let external_path_to_valid_external_path_pre #bytes #cb #tkt #l #i #li t p group_id =
   let lp = get_external_path_leaf p in
   compute_leaf_parent_hash_from_external_path_pre t p (length #bytes (root_parent_hash #bytes)) &&
-  lp.data.source = LNS_update () && li < pow2 32 && (
-    let tbs_length = ((prefixes_length #bytes ((ps_leaf_node_tbs_nt tkt).serialize ({data = lp.data; group_id; leaf_index = li;}))) + 2 + (hash_length #bytes)) in
+  lp.source = LNS_update () && li < pow2 32 && (
+    let tbs_length = ((prefixes_length #bytes ((ps_leaf_node_tbs_nt tkt).serialize ({data = lp; group_id; leaf_index = li;}))) + 2 + (hash_length #bytes)) in
     tbs_length < pow2 30 &&
     sign_with_label_pre #bytes "LeafNodeTBS" tbs_length
   )
 
 #push-options "--z3rlimit 50"
-val external_path_to_valid_external_path: #bytes:Type0 -> {|crypto_bytes bytes|} -> #tkt:treekem_types bytes -> #l:nat -> #i:tree_index l -> #li:leaf_index l i -> t:treesync bytes tkt l i -> p:external_pathsync bytes tkt l i li -> group_id:mls_bytes bytes -> sign_private_key bytes -> sign_nonce bytes -> Pure (external_pathsync bytes tkt l i li)
+val external_path_to_valid_external_path: #bytes:Type0 -> {|crypto_bytes bytes|} -> #tkt:treekem_types bytes -> #l:nat -> #i:tree_index l -> #li:leaf_index l i -> t:treesync bytes tkt l i -> p:external_pathsync bytes tkt l i li -> group_id:mls_bytes bytes -> sign_private_key bytes -> sign_nonce bytes -> Pure (pathsync bytes tkt l i li)
   (requires external_path_to_valid_external_path_pre t p group_id)
   (ensures fun _ -> True)
 let external_path_to_valid_external_path #bytes #cb #tkt #l #i #li t p group_id sign_key nonce =
   let computed_parent_hash = compute_leaf_parent_hash_from_external_path t p root_parent_hash in
   let lp = get_external_path_leaf p in
-  let new_lp_data = { lp.data with source = LNS_commit (); parent_hash = computed_parent_hash; } in
+  let new_lp_data = { lp with source = LNS_commit (); parent_hash = computed_parent_hash; } in
   let new_lp_tbs: bytes = serialize (leaf_node_tbs_nt bytes tkt) ({data = new_lp_data; group_id; leaf_index = li;}) in
   let new_signature = sign_with_label sign_key "LeafNodeTBS" new_lp_tbs nonce in
-  set_external_path_leaf p ({ data = new_lp_data; signature = new_signature })
+  set_external_path_leaf p ({ data = new_lp_data; signature = new_signature } <: leaf_node_nt bytes tkt)
 #pop-options
 
-val apply_external_path_aux_pre: #bytes:Type0 -> {|crypto_bytes bytes|} -> #tkt:treekem_types bytes -> #l:nat -> #i:tree_index l -> #li:leaf_index l i -> t:treesync bytes tkt l i -> external_pathsync bytes tkt l i li -> mls_nat -> bool
+val apply_external_path_aux_pre: #bytes:Type0 -> {|crypto_bytes bytes|} -> #tkt:treekem_types bytes -> #l:nat -> #i:tree_index l -> #li:leaf_index l i -> t:treesync bytes tkt l i -> pathsync bytes tkt l i li -> mls_nat -> bool
 let rec apply_external_path_aux_pre #bytes #cb #tkt #l #i #li t p length_parent_parent_hash =
   match t, p with
   | TLeaf _, PLeaf _ -> true
@@ -212,7 +212,7 @@ let rec apply_external_path_aux_pre #bytes #cb #tkt #l #i #li t p length_parent_
       else apply_external_path_aux_pre right p_next new_length_parent_parent_hash
     )
 
-val apply_external_path_aux: #bytes:Type0 -> {|crypto_bytes bytes|} -> #tkt:treekem_types bytes -> #l:nat -> #i:tree_index l -> #li:leaf_index l i -> t:treesync bytes tkt l i -> p:external_pathsync bytes tkt l i li -> parent_parent_hash:mls_bytes bytes -> Pure (treesync bytes tkt l i)
+val apply_external_path_aux: #bytes:Type0 -> {|crypto_bytes bytes|} -> #tkt:treekem_types bytes -> #l:nat -> #i:tree_index l -> #li:leaf_index l i -> t:treesync bytes tkt l i -> p:pathsync bytes tkt l i li -> parent_parent_hash:mls_bytes bytes -> Pure (treesync bytes tkt l i)
   (requires apply_external_path_aux_pre t p (length #bytes parent_parent_hash))
   (ensures fun _ -> True)
 let rec apply_external_path_aux #bytes #cb #tkt #l #i #li t p parent_parent_hash =
@@ -227,11 +227,11 @@ let rec apply_external_path_aux #bytes #cb #tkt #l #i #li t p parent_parent_hash
       TNode new_opt_content left (apply_external_path_aux right p_next new_parent_parent_hash)
     )
 
-val apply_external_path_pre: #bytes:Type0 -> {|crypto_bytes bytes|} -> #tkt:treekem_types bytes -> #l:nat -> #li:leaf_index l 0 -> t:treesync bytes tkt l 0 -> external_pathsync bytes tkt l 0 li -> bool
+val apply_external_path_pre: #bytes:Type0 -> {|crypto_bytes bytes|} -> #tkt:treekem_types bytes -> #l:nat -> #li:leaf_index l 0 -> t:treesync bytes tkt l 0 -> pathsync bytes tkt l 0 li -> bool
 let apply_external_path_pre #bytes #cb #tkt #l #li t p =
   apply_external_path_aux_pre t p (length #bytes (root_parent_hash #bytes))
 
-val apply_external_path: #bytes:Type0 -> {|crypto_bytes bytes|} -> #tkt:treekem_types bytes -> #l:nat -> #li:leaf_index l 0 -> t:treesync bytes tkt l 0 -> p:external_pathsync bytes tkt l 0 li -> Pure (treesync bytes tkt l 0)
+val apply_external_path: #bytes:Type0 -> {|crypto_bytes bytes|} -> #tkt:treekem_types bytes -> #l:nat -> #li:leaf_index l 0 -> t:treesync bytes tkt l 0 -> p:pathsync bytes tkt l 0 li -> Pure (treesync bytes tkt l 0)
   (requires apply_external_path_pre t p)
   (ensures fun _ -> True)
 let apply_external_path #bytes #cb #tkt #l #li t p =
