fstar/MLS.TreeSync.Types.fst
@@ -7,5 +7,8 @@ open MLS.TreeSync.NetworkTypes
 let treesync (bytes:Type0) {|bytes_like bytes|} (tkt:treekem_types bytes) =
   tree (option (leaf_node_nt bytes tkt)) (option (parent_node_nt bytes tkt))
 
-let external_pathsync (bytes:Type0) {|bytes_like bytes|} (tkt:treekem_types bytes) =
+let pathsync (bytes:Type0) {|bytes_like bytes|} (tkt:treekem_types bytes) =
   path (leaf_node_nt bytes tkt) (option tkt.node_content)
+
+let external_pathsync (bytes:Type0) {|bytes_like bytes|} (tkt:treekem_types bytes) =
+  path (leaf_node_data_nt bytes tkt) (option tkt.node_content)
